Work towards a fix of the not-ok executions diverging

vale/code/lib/transformers/Vale.Transformers.InstructionReorder.fst
@@ -496,8 +496,12 @@ let run2 (f1 f2:st unit) (s:machine_state) : machine_state =
   let open Vale.X64.Machine_Semantics_s in
   run (f1;; f2;; return ()) s
 
+let equiv_states_or_both_not_ok (s1 s2:machine_state) =
+  (equiv_states s1 s2) \/
+  ((not s1.ms_ok) /\ (not s2.ms_ok))
+
 let commutes (s:machine_state) (f1 f2:st unit) : GTot Type0 =
-  equiv_states
+  equiv_states_or_both_not_ok
     (run2 f1 f2 s)
     (run2 f2 f1 s)
 
@@ -689,36 +693,38 @@ let lemma_commute (f1 f2:st unit) (r1 w1 r2 w2:list location) (s:machine_state) 
         (bounded_effects r2 w2 f2) /\
         !!(rw_exchange_allowed (r1, w1) (r2, w2))))
     (ensures (
-        equiv_states
+        equiv_states_or_both_not_ok
           (run2 f1 f2 s)
           (run2 f2 f1 s))) =
   let s12 = run2 f1 f2 s in
   let s21 = run2 f2 f1 s in
-  let is1 = run f1 s in
-  let is2 = run f2 s in
-  let is12 = run f2 is1 in
-  let is21 = run f1 is2 in
-  lemma_disjoint_implies_unchanged_at r1 w2 s is2;
-  lemma_disjoint_implies_unchanged_at r2 w1 s is1;
-  assert (unchanged_at w1 is1 is21);
-  assert (unchanged_at w2 is2 is12);
-  assert (unchanged_except w2 s is2);
-  assert (unchanged_except w1 s is1);
-  assert (unchanged_except w2 is1 is12);
-  assert (unchanged_except w1 is2 is21);
-  lemma_unchanged_except_transitive w1 w2 s is1 is12;
-  assert (unchanged_except (w1 `L.append` w2) s is12);
-  lemma_unchanged_except_transitive w2 w1 s is2 is21;
-  assert (unchanged_except (w2 `L.append` w1) s is21);
-  lemma_unchanged_except_append_symmetric w1 w2 s is12;
-  lemma_unchanged_except_append_symmetric w2 w1 s is21;
-  lemma_unchanged_except_same_transitive (w1 `L.append` w2) s is12 is21;
-  lemma_unchanged_at_combine w1 w2 is1 is2 is12 is21;
-  lemma_unchanged_at_and_except (w1 `L.append` w2) is12 is21;
-  assert (unchanged_except [] is12 is21);
-  assert (s21.ms_ok = s12.ms_ok);
-  lemma_equiv_states_when_except_none is12 is21 s12.ms_ok;
-  assert (equiv_states (run2 f1 f2 s) (run2 f2 f1 s))
+  if not s12.ms_ok && not s21.ms_ok then () else (
+    let is1 = run f1 s in
+    let is2 = run f2 s in
+    let is12 = run f2 is1 in
+    let is21 = run f1 is2 in
+    lemma_disjoint_implies_unchanged_at r1 w2 s is2;
+    lemma_disjoint_implies_unchanged_at r2 w1 s is1;
+    assert (unchanged_at w1 is1 is21);
+    assert (unchanged_at w2 is2 is12);
+    assert (unchanged_except w2 s is2);
+    assert (unchanged_except w1 s is1);
+    assert (unchanged_except w2 is1 is12);
+    assert (unchanged_except w1 is2 is21);
+    lemma_unchanged_except_transitive w1 w2 s is1 is12;
+    assert (unchanged_except (w1 `L.append` w2) s is12);
+    lemma_unchanged_except_transitive w2 w1 s is2 is21;
+    assert (unchanged_except (w2 `L.append` w1) s is21);
+    lemma_unchanged_except_append_symmetric w1 w2 s is12;
+    lemma_unchanged_except_append_symmetric w2 w1 s is21;
+    lemma_unchanged_except_same_transitive (w1 `L.append` w2) s is12 is21;
+    lemma_unchanged_at_combine w1 w2 is1 is2 is12 is21;
+    lemma_unchanged_at_and_except (w1 `L.append` w2) is12 is21;
+    assert (unchanged_except [] is12 is21);
+    assert (s21.ms_ok = s12.ms_ok);
+    lemma_equiv_states_when_except_none is12 is21 s12.ms_ok;
+    assert (equiv_states (run2 f1 f2 s) (run2 f2 f1 s))
+  )
 
 let lemma_machine_eval_ins_st_exchange (i1 i2 : ins) (s : machine_state) :
   Lemma
@@ -741,7 +747,7 @@ let lemma_instruction_exchange' (i1 i2 : ins) (s1 s2 : machine_state) :
         (let s1', s2' =
            machine_eval_ins i2 (machine_eval_ins i1 s1),
            machine_eval_ins i1 (machine_eval_ins i2 s2) in
-         equiv_states s1' s2'))) =
+         equiv_states_or_both_not_ok s1' s2'))) =
   lemma_machine_eval_ins_st_exchange i1 i2 s1;
   lemma_eval_ins_equiv_states i2 s1 s2;
   lemma_eval_ins_equiv_states i1 (machine_eval_ins i2 s1) (machine_eval_ins i2 s2)
@@ -755,7 +761,7 @@ let lemma_instruction_exchange (i1 i2 : ins) (s1 s2 : machine_state) :
         (let s1', s2' =
            machine_eval_ins i2 (filt_state (machine_eval_ins i1 (filt_state s1))),
            machine_eval_ins i1 (filt_state (machine_eval_ins i2 (filt_state s2))) in
-         equiv_states s1' s2'))) =
+         equiv_states_or_both_not_ok s1' s2'))) =
   lemma_eval_ins_equiv_states i1 s1 (filt_state s1);
   lemma_eval_ins_equiv_states i2 s2 (filt_state s2);
   lemma_eval_ins_equiv_states i2 (machine_eval_ins i1 (filt_state s1)) (filt_state (machine_eval_ins i1 (filt_state s1)));
@@ -784,7 +790,7 @@ let lemma_code_exchange (c1 c2 : code) (fuel:nat) (s1 s2 : machine_state) :
         (let Some s1', Some s2' =
            machine_eval_codes [c1; c2] fuel s1,
            machine_eval_codes [c2; c1] fuel s2 in
-         equiv_states s1' s2'))) =
+         equiv_states_or_both_not_ok s1' s2'))) =
   let Some s1', Some s2' =
     machine_eval_codes [c1; c2] fuel s1,
     machine_eval_codes [c2; c1] fuel s2 in
@@ -813,8 +819,8 @@ let lemma_code_exchange (c1 c2 : code) (fuel:nat) (s1 s2 : machine_state) :
     // assert_norm (equiv_states s23 s24);
     assert (equiv_states s2' s24);
     lemma_instruction_exchange i1 i2 s1 s2;
-    assert (equiv_states s14 s24);
-    assert (equiv_states s1' s2')
+    assert (equiv_states_or_both_not_ok s14 s24);
+    assert (equiv_states_or_both_not_ok s1' s2')
   | _ -> ()
 #pop-options
 
@@ -905,6 +911,7 @@ let rec lemma_bubble_to_top (cs : codes) (i:nat{i < L.length cs}) (fuel:nat) (s 
     let Some s_start = machine_eval_code (L.hd cs) fuel s in
     let Some s_0' = machine_eval_code x fuel s_start in
     let Some s_0'' = machine_eval_code (L.hd cs) fuel s_0 in
+    admit (); (* TODO FIXME Broke due to change of [equiv_states_or_both_not_ok] *)
     assert (equiv_states s_0' s_0'');
     lemma_eval_codes_equiv_states tlxs fuel s_0' s_0'';
     let Some s_1' = machine_eval_codes tlxs fuel s_0' in
